DY/Bytes/AttackerKnowledge.lean
@@ -1,0 +1,293 @@
+/-
+  This module allows to define modularly
+  the computations that may perform a Dolev-Yao attacker.
+-/
+
+module
+
+public import DY.Kleene
+public import DY.Bytes.Basic
+public import DY.Trace.Basic
+
+
+namespace DY
+
+variable [BytesFunctor]
+
+/--
+  The attacker knowledge is ultimately defined as a Kleene fixpoint,
+  and `SubAttackerKnowledge` is a component of this fixpoint computation.
+
+  For example, to say that the attacker is allowed to concatenate bytes,
+  we can write:
+
+    -- attacker knows `out` when
+    pred p out :=
+      ∃ lhs rhs,
+        -- `out` is the concatenation of `lhs` and `rhs` and
+        out = concat lhs rhs ∧
+        p lhs ∧ -- the attacker knows lhs and
+        p rhs   -- the attacker knows rhs.
+
+  To prove the scott-continuity of `pred` (a technical requirement for Kleene fixpoint)
+  it is better to use the `Forall` predicate like this:
+
+    pred p out :=
+      ∃ lhs rhs,
+        out = concat lhs rhs ∧
+        DY.Kleene.Forall p [lhs, rhs]
+
+  This allows to rely on the lemma `DY.Kleene.isScottContinuous_Forall_lemma`,
+  and allow for `pred_isScottContinuous` to be proved automatically by our tactic script.
+
+  The `SubF` parameter is not useful in this definition.
+  It is only for hygiene, to make sure we don't miss equational theories
+  by using `SubAttackerKnowledge.combine`
+-/
+
+public
+structure SubAttackerKnowledge (SubF: Type → Type) where
+  pred: (Bytes → Prop) → Bytes → Prop
+  pred_isScottContinuous: DY.Kleene.IsScottContinuous pred := by
+    intro chain h_chain
+    funext buf
+    simp only [eq_iff_iff]
+    constructor
+    · try simp [DY.Kleene.isScottContinuous_Forall_lemma chain h_chain]
+      try simp [DY.Kleene.Chain.union, DY.Kleene.Chain.map]
+      try grind
+    · try simp [DY.Kleene.Forall, DY.Kleene.Chain.union, DY.Kleene.Chain.map]
+      try grind
+
+public
+class AttackerKnowledge where
+  attackerKnowledge: SubAttackerKnowledge BytesF
+
+public
+class AttackerKnowledge.HasStep
+  {SubF1: Type → Type}
+  {SubF2: semiOutParam (Type → Type)}
+  (att1: SubAttackerKnowledge SubF1)
+  (att2: semiOutParam (SubAttackerKnowledge SubF2))
+where
+  pf: ∀ p b, att1.pred p b → att2.pred p b
+
+public
+class AttackerKnowledge.Has
+  [AttackerKnowledge]
+  {SubF: Type → Type}
+  (att: SubAttackerKnowledge SubF)
+where
+  pf: ∀ p b, att.pred p b → AttackerKnowledge.attackerKnowledge.pred p b
+
+namespace AttackerKnowledge
+
+public
+instance
+  [AttackerKnowledge]
+  : AttackerKnowledge.Has AttackerKnowledge.attackerKnowledge
+where
+  pf p b := by simp
+
+public
+instance
+  [AttackerKnowledge]
+  {SubF1 SubF2: Type → Type}
+  (att1: SubAttackerKnowledge SubF1)
+  (att2: SubAttackerKnowledge SubF2)
+  [inst1: AttackerKnowledge.HasStep att1 att2]
+  [inst2: AttackerKnowledge.Has att2]
+  : AttackerKnowledge.Has att1
+where
+  pf p b := by simp_all [inst1.pf, inst2.pf]
+
+end AttackerKnowledge
+
+public
+def SubAttackerKnowledge.combine
+  {t: Type}
+  {SubFs: t → Type → Type}
+  (atts: ∀ id, SubAttackerKnowledge (SubFs id))
+  : SubAttackerKnowledge (BytesFunctor.combine SubFs)
+where
+  pred := DY.Kleene.combine (fun id => (atts id).pred)
+  pred_isScottContinuous := DY.Kleene.combine_isScottContinuous (fun id => (atts id).pred) (fun id => (atts id).pred_isScottContinuous)
+
+public
+def SubAttackerKnowledge.combine'
+  {SubF: Type → Type}
+  {t: Type}
+  (atts: t → SubAttackerKnowledge SubF)
+  : SubAttackerKnowledge SubF
+where
+  pred := DY.Kleene.combine (fun id => (atts id).pred)
+  pred_isScottContinuous := DY.Kleene.combine_isScottContinuous (fun id => (atts id).pred) (fun id => (atts id).pred_isScottContinuous)
+
+@[expose]
+public
+def SubAttackerKnowledge.fromPred {SubF: Type → Type} (pred: Bytes → Prop): SubAttackerKnowledge SubF where
+  pred p buf := pred buf
+
+namespace AttackerKnowledge
+
+public
+instance
+  {t: Type}
+  {SubFs: t → Type → Type}
+  (atts: (id: t) → SubAttackerKnowledge (SubFs id))
+  (id: t)
+  : AttackerKnowledge.HasStep (atts id) (SubAttackerKnowledge.combine atts)
+where
+  pf p b := by
+    simp [SubAttackerKnowledge.combine, Kleene.combine]
+    intro
+    exists id
+
+public
+instance
+  {SubF: Type → Type}
+  {t: Type}
+  (atts: t → SubAttackerKnowledge SubF)
+  (id: t)
+  : AttackerKnowledge.HasStep (atts id) (SubAttackerKnowledge.combine' atts)
+where
+  pf p b := by
+    simp [SubAttackerKnowledge.combine', Kleene.combine]
+    intro
+    exists id
+
+end AttackerKnowledge
+
+-- TODO
+public
+opaque Trace.MessageSent (tr: Trace α) (b: Bytes): Prop
+public
+axiom Trace.MessageSent_erase (tr: Trace α) (b: Bytes): tr.MessageSent b = tr.erase.MessageSent b
+
+@[expose]
+public
+def Bytes.AttackerKnows.baseKnowledge (tr: Trace α): SubAttackerKnowledge BytesF :=
+  SubAttackerKnowledge.fromPred tr.MessageSent
+
+def Bytes.AttackerKnows.attackerKnowledge [AttackerKnowledge] (tr: Trace α): SubAttackerKnowledge BytesF :=
+  SubAttackerKnowledge.combine' (fun (id: Fin 2) =>
+    match id with
+    | 0 => AttackerKnowledge.attackerKnowledge
+    | 1 => baseKnowledge tr
+  )
+
+public
+def Bytes.AttackerKnows [AttackerKnowledge] (b: Bytes) (tr: Trace α): Prop :=
+  Kleene.mkWeakestFixpoint ((Bytes.AttackerKnows.attackerKnowledge tr).pred) b
+
+def Bytes.AttackerKnows.attackerKnow.prove
+  [AttackerKnowledge]
+  {SubF: Type → Type}
+  (att: SubAttackerKnowledge SubF)
+  [inst: AttackerKnowledge.Has att]
+  (p: Bytes → Prop)
+  (b: Bytes) (tr: Trace α)
+  : att.pred p b → (Bytes.AttackerKnows.attackerKnowledge tr).pred p b
+:= by
+  unfold Bytes.AttackerKnows.attackerKnowledge SubAttackerKnowledge.combine' Kleene.combine
+  have := inst.pf p b
+  simp
+  grind
+
+/--
+  Main theorem to prove that the attacker knows some particular value
+-/
+public
+theorem Bytes.AttackerKnows.prove
+  [AttackerKnowledge]
+  {SubF: Type → Type}
+  (att: SubAttackerKnowledge SubF)
+  [AttackerKnowledge.Has att]
+  (b: Bytes) (tr: Trace α)
+  : att.pred (Bytes.AttackerKnows · tr) b →
+    Bytes.AttackerKnows b tr
+:= by
+  intro h
+  have h1 := Bytes.AttackerKnows.attackerKnow.prove att (Bytes.AttackerKnows · tr) b tr h
+  have h2 := Kleene.mkWeakestFixpoint_is_fixpoint (Bytes.AttackerKnows.attackerKnowledge tr).pred (Bytes.AttackerKnows.attackerKnowledge tr).pred_isScottContinuous
+  unfold Bytes.AttackerKnows at *
+  grind
+
+/--
+  The attacker knowledge `AttackerKnows` is the weakest predicate `P` such that every sub-attacker knowledge predicate `att`,
+    att.pred P b
+  implies
+    P b
+
+  The attacker knowledge satisfies this property: this is the theorem by `Bytes.AttackerKnows.prove`
+  The attacker knowledge is the weakest predicate: this is the theorem `Bytes.AttackerKnows.is_least_fixpoint`.
+  In other words, if a predicate `P` has this property, then `Bytes.AttackerKnows b => P b`
+
+  We can use `SubAttackerKnowledge.Implies` to modularly prove that a predicate `P` satisfy this property.
+-/
+@[expose]
+public
+def SubAttackerKnowledge.Implies {SubF: Type → Type} (att: SubAttackerKnowledge SubF) (p: Bytes → Prop): Prop :=
+  ∀ b, att.pred p b → p b
+
+public
+theorem SubAttackerKnowledge.combine'.implies
+  {SubF: Type → Type}
+  {t: Type}
+  (atts: t → SubAttackerKnowledge SubF)
+  (p: Bytes → Prop)
+  (pfs: ∀ id, SubAttackerKnowledge.Implies (atts id) p)
+  : SubAttackerKnowledge.Implies (SubAttackerKnowledge.combine' atts) p
+:= by
+  intro b
+  simp only [SubAttackerKnowledge.combine', Kleene.combine, forall_exists_index]
+  intro id
+  exact pfs id b
+
+public
+theorem SubAttackerKnowledge.combine.implies
+  {t: Type}
+  {SubFs: t → Type → Type}
+  (atts: ∀ id, SubAttackerKnowledge (SubFs id))
+  (p: Bytes → Prop)
+  (pfs: ∀ id, SubAttackerKnowledge.Implies (atts id) p)
+  : SubAttackerKnowledge.Implies (SubAttackerKnowledge.combine atts) p
+:= by
+  intro b
+  simp only [SubAttackerKnowledge.combine, Kleene.combine, forall_exists_index]
+  intro id
+  exact pfs id b
+
+public
+theorem Bytes.AttackerKnows.is_least_fixpoint
+  [AttackerKnowledge]
+  (pred: Bytes → Prop)
+  (b: Bytes) (tr: Trace α)
+  (pf1: SubAttackerKnowledge.Implies AttackerKnowledge.attackerKnowledge pred)
+  (pf2: SubAttackerKnowledge.Implies (Bytes.AttackerKnows.baseKnowledge tr) pred)
+  : Bytes.AttackerKnows b tr →
+    pred b
+:=
+  Kleene.mkWeakestFixpoint_is_weakest ((Bytes.AttackerKnows.attackerKnowledge tr).pred) ((Bytes.AttackerKnows.attackerKnowledge tr).pred_isScottContinuous) pred (by
+    simp [Subset, attackerKnowledge, SubAttackerKnowledge.combine', Kleene.combine]
+    intro b
+    have := pf1 b
+    have := pf2 b
+    grind
+  ) b
+
+public
+theorem Bytes.AttackerKnows.pred_trace_erase [AttackerKnowledge] (tr: Trace α) (b: Bytes):
+  b.AttackerKnows tr = b.AttackerKnows (tr.erase)
+:= by
+  simp only [Bytes.AttackerKnows, Bytes.AttackerKnows.attackerKnowledge]
+  congr
+  funext
+  split
+  · rfl
+  · simp only [Bytes.AttackerKnows.baseKnowledge]
+    congr 1
+    funext
+    apply Trace.MessageSent_erase
+
+end DY
