DY/Bytes/AttackerKnowledgeTheorem.lean
@@ -1,0 +1,81 @@
+/-
+  This module allows to modularly prove the attacker knowledge theorem:
+  this is a key theorem in the DyLean methodology,
+  saying for traces that satisfy the trace invariant,
+  if the attacker knows a `Bytes`,
+  then this `Bytes` must be publishable.
+-/
+
+module
+
+public import DY.Bytes.Basic
+public import DY.Bytes.Invariants
+public import DY.Bytes.AttackerKnowledge
+public import DY.Trace
+
+
+namespace DY
+
+variable [BytesFunctor]
+variable [BytesInvariants]
+
+public
+class SubAttackerKnowledgeTheorem {SubF: Type → Type} (att: SubAttackerKnowledge SubF) where
+  pf: ∀ b: Bytes, ∀ tr: ProofTrace, tr.invariant → att.pred (·.Publishable tr) b → b.Publishable tr
+
+public
+class AttackerKnowledgeTheorem [AttackerKnowledge] where
+  inst: SubAttackerKnowledgeTheorem (AttackerKnowledge.attackerKnowledge)
+
+section AttackerKnowledgeTheorem
+
+public
+instance
+  {SubF: Type → Type}
+  {t: Type}
+  (atts: t → SubAttackerKnowledge SubF)
+  [pfs: ∀ id, SubAttackerKnowledgeTheorem (atts id)]
+  : SubAttackerKnowledgeTheorem (SubAttackerKnowledge.combine' atts)
+where
+  pf := by
+    intro b tr h_tr
+    apply SubAttackerKnowledge.combine'.implies
+    intro id b
+    exact (pfs id).pf b tr h_tr
+
+public
+instance
+  {t: Type}
+  {SubFs: t → Type → Type}
+  (atts: ∀ id, SubAttackerKnowledge (SubFs id))
+  [pfs: ∀ id, SubAttackerKnowledgeTheorem (atts id)]
+  : SubAttackerKnowledgeTheorem (SubAttackerKnowledge.combine atts)
+where
+  pf := by
+    intro b tr h_tr
+    apply SubAttackerKnowledge.combine.implies
+    intro id b
+    exact (pfs id).pf b tr h_tr
+
+end AttackerKnowledgeTheorem
+
+public
+axiom Bytes.MessageSent_implies_Publishable (b: Bytes) (tr: ProofTrace): tr.invariant → tr.MessageSent b → b.Publishable tr
+
+public
+theorem Bytes.AttackerKnows_implies_Publishable
+  [AttackerKnowledge]
+  [inst: AttackerKnowledgeTheorem]
+  (b: Bytes) (tr: ProofTrace)
+  : tr.invariant →
+    Bytes.AttackerKnows b tr →
+    b.Publishable tr
+:= by
+  intro h_tr
+  apply Bytes.AttackerKnows.is_least_fixpoint (·.Publishable tr) b tr
+  · intro b
+    exact inst.inst.pf b tr h_tr
+  · intro b
+    exact Bytes.MessageSent_implies_Publishable b tr h_tr
+
+end DY
