DY/EquationalTheory/Concat.lean
@@ -1,0 +1,326 @@
+module
+
+public import DY.Bytes
+public import DY.Misc.Instances
+
+namespace DY.Concat
+
+public
+class CanConcat (Bytes: Type u) where
+  concat: Bytes → Bytes → Bytes
+  split: Bytes → Nat → Option (Bytes × Bytes)
+
+export CanConcat (concat)
+export CanConcat (split)
+
+section Constructors
+
+public
+structure Concat (Bytes: Type) where
+  lhs: Bytes
+  rhs: Bytes
+
+public
+instance: ALaCarte.FunctorSizeOf Concat where
+  sizeOf | {lhs, rhs} => sizeOf lhs + sizeOf rhs
+
+public
+instance: ALaCarte.Representable Concat where
+  CtorId := Unit
+  ctors | () => { Data := Unit, nRec := 2 }
+
+  toRepr | {lhs, rhs} => {
+    id := ()
+    data := ()
+    as := #v[lhs, rhs]
+  }
+  fromRepr
+  | {id, data, as} =>
+    let lhs := as[0]
+    let rhs := as[1]
+    { lhs, rhs }
+  from_to | {lhs, rhs} => by rfl
+  to_from
+  | {id, data, as} => by
+    simp_all <;> grind
+  sizeOf_eq | {lhs, rhs} => by simp +arith [ALaCarte.FunctorSizeOf.sizeOf]
+
+public instance: ALaCarte.RepresentableDecidableEq Concat where
+public instance: ALaCarte.RepresentableOrd Concat where
+public instance: SubBytesFunctor Concat where
+
+public
+abbrev SubF := Concat
+
+public
+def Concat.length [BytesFunctor]: Bytes.PartialLength Concat :=
+  fun { lhs, rhs } rec =>
+    rec lhs + rec rhs
+
+public
+abbrev SubF.length [BytesFunctor]: Bytes.PartialLength SubF := Concat.length
+
+variable [BytesFunctor] [BytesFunctor.Has SubF]
+variable [BytesLength]
+
+public
+abbrev Concat.pack (x: Concat Bytes) := BytesView.pack x
+
+public
+instance: CanConcat Bytes where
+  concat lhs rhs := ({lhs, rhs}: Concat Bytes).pack
+
+  split buf i :=
+    match buf.view? Concat with
+    | some ({ lhs, rhs }) =>
+      if lhs.length = i then
+        some (lhs, rhs)
+      else
+        none
+    | none => none
+
+public
+theorem split_concat
+  (lhs rhs: Bytes)
+  : split (concat lhs rhs) (lhs.length) = some (lhs, rhs)
+:= by
+  simp only [split, concat]
+  grind
+
+public
+theorem concat_split
+  (buf: Bytes) (i: Nat) (lhs rhs: Bytes)
+  : split buf i = some (lhs, rhs) → concat lhs rhs = buf
+:= by
+  simp only [concat, split]
+  grind
+
+end Constructors
+
+section AttackerKnowledge
+
+variable [BytesFunctor] [BytesFunctor.Has SubF]
+variable [BytesLength]
+
+public
+def attKnowsConcat: SubAttackerKnowledge Concat where
+  pred p out :=
+    ∃ lhs rhs,
+      out = concat lhs rhs ∧
+      DY.Kleene.Forall p [lhs, rhs]
+
+public
+def attKnowsSplitLeft: SubAttackerKnowledge Concat where
+  pred p out :=
+    ∃ inp rhs i,
+      some (out, rhs) = split inp i ∧
+      DY.Kleene.Forall p [inp]
+
+public
+def attKnowsSplitRight: SubAttackerKnowledge Concat where
+  pred p out :=
+    ∃ inp lhs i,
+      some (lhs, out) = split inp i ∧
+      DY.Kleene.Forall p [inp]
+
+def attackerKnowledge.internal (id: Fin 3): SubAttackerKnowledge Concat :=
+  match id with
+  | 0 => attKnowsConcat
+  | 1 => attKnowsSplitLeft
+  | 2 => attKnowsSplitRight
+
+public
+def attackerKnowledge: SubAttackerKnowledge Concat :=
+  SubAttackerKnowledge.combine' attackerKnowledge.internal
+
+public instance: AttackerKnowledge.HasStep attKnowsConcat attackerKnowledge := inferInstanceAs (AttackerKnowledge.HasStep (attackerKnowledge.internal 0) (SubAttackerKnowledge.combine' attackerKnowledge.internal))
+public instance: AttackerKnowledge.HasStep attKnowsSplitLeft attackerKnowledge := inferInstanceAs (AttackerKnowledge.HasStep (attackerKnowledge.internal 1) (SubAttackerKnowledge.combine' attackerKnowledge.internal))
+public instance: AttackerKnowledge.HasStep attKnowsSplitRight attackerKnowledge := inferInstanceAs (AttackerKnowledge.HasStep (attackerKnowledge.internal 2) (SubAttackerKnowledge.combine' attackerKnowledge.internal))
+
+variable [AttackerKnowledge] [AttackerKnowledge.Has attackerKnowledge]
+
+public
+theorem attacker_knows_concat
+  (lhs rhs: Bytes) (tr: Trace α)
+  : lhs.AttackerKnows tr →
+    rhs.AttackerKnows tr →
+    (concat lhs rhs).AttackerKnows tr
+:= by
+  intro h_lhs h_rhs
+  apply Bytes.AttackerKnows.prove attKnowsConcat
+  simp only [attKnowsConcat, Kleene.Forall]
+  grind
+
+public
+theorem attacker_knows_split
+  (buf: Bytes) (i: Nat) (tr: Trace α)
+  : buf.AttackerKnows tr →
+    match split buf i with
+    | none => True
+    | some (lhs, rhs) =>
+      lhs.AttackerKnows tr ∧
+      rhs.AttackerKnows tr
+:= by
+  intro h_buf
+  split
+  · trivial
+  rename_i lhs rhs _
+  constructor
+  · apply Bytes.AttackerKnows.prove attKnowsSplitLeft
+    simp only [attKnowsSplitLeft, Kleene.Forall]
+    grind
+  · apply Bytes.AttackerKnows.prove attKnowsSplitRight
+    simp only [attKnowsSplitRight, Kleene.Forall]
+    grind
+
+end AttackerKnowledge
+
+section Invariants
+
+variable [BytesFunctor] [BytesFunctor.Has SubF]
+
+public
+def Concat.invariants: Bytes.PartialInvariants Concat where
+  well_formed := fun {lhs, rhs} rec tr =>
+    (rec lhs) tr ∧ (rec rhs) tr
+
+  usage := fun {lhs, rhs} rec tr => Usage.nothing
+
+  label := fun {lhs, rhs} rec tr =>
+    Label.meet ((rec lhs) tr) ((rec rhs) tr)
+
+  invariant := fun {lhs, rhs} rec tr =>
+    (rec lhs) tr ∧ (rec rhs) tr
+
+public
+abbrev invariants: Bytes.PartialInvariants SubF := Concat.Concat.invariants
+
+public
+def Concat.invariantsProofs [BytesInvariants]: Bytes.PartialInvariantsProofs Concat.invariants where
+
+public
+abbrev invariantsProofs [BytesInvariants]: Bytes.PartialInvariantsProofs invariants := Concat.Concat.invariantsProofs
+
+variable [BytesInvariants] [BytesInvariants.Has invariants]
+variable [BytesLength]
+
+@[simp]
+public
+theorem concat.WellFormed
+  (lhs rhs: Bytes) (tr: ProofTrace)
+  : (concat lhs rhs).WellFormed tr = (lhs.WellFormed tr ∧ rhs.WellFormed tr)
+:= by
+  simp [concat, Bytes.WellFormed.eq, Concat.invariants]
+
+@[simp]
+public
+theorem concat.label
+  (lhs rhs: Bytes) (tr: ProofTrace)
+  : (concat lhs rhs).label tr = Label.meet (lhs.label tr) (rhs.label tr)
+:= by
+  simp [concat, Bytes.label.eq, Concat.invariants]
+
+@[simp]
+public
+theorem concat.Invariant
+  (lhs rhs: Bytes) (tr: ProofTrace)
+  : (concat lhs rhs).Invariant tr = (lhs.Invariant tr ∧ rhs.Invariant tr)
+:= by
+  simp [concat, Bytes.Invariant.eq, Concat.invariants]
+
+@[simp]
+public
+theorem split.WellFormed
+  (buf: Bytes) (i: Nat) (tr: ProofTrace)
+  : match split buf i with
+    | none => True
+    | some (lhs, rhs) =>
+      buf.WellFormed tr = (lhs.WellFormed tr ∧ rhs.WellFormed tr)
+:= by
+  split
+  · trivial
+  rename_i lhs rhs heq
+  rewrite [← concat_split buf i lhs rhs heq]
+  simp
+
+@[simp]
+public
+theorem split.label
+  (buf: Bytes) (i: Nat) (tr: ProofTrace)
+  : match split buf i with
+    | none => True
+    | some (lhs, rhs) =>
+      buf.label tr = Label.meet (lhs.label tr) (rhs.label tr)
+:= by
+  split
+  · trivial
+  rename_i lhs rhs heq
+  rewrite [← concat_split buf i lhs rhs heq]
+  simp
+
+@[simp]
+public
+theorem split.Invariant
+  (buf: Bytes) (i: Nat) (tr: ProofTrace)
+  : buf.Invariant tr →
+    match split buf i with
+    | none => True
+    | some (lhs, rhs) =>
+      lhs.Invariant tr ∧ rhs.Invariant tr
+:= by
+  intro h_buf
+  split
+  · trivial
+  rename_i lhs rhs heq
+  rewrite [← concat_split buf i lhs rhs heq] at h_buf
+  simp_all
+
+end Invariants
+
+section AttackerKnowledgeTheorem
+
+variable [BytesFunctor] [BytesInvariants]
+variable [BytesFunctor.Has SubF]
+variable [BytesLength]
+variable [BytesInvariants.Has invariants]
+
+instance: SubAttackerKnowledgeTheorem attKnowsConcat where
+  pf := by
+    simp only [attKnowsConcat]
+    intro out tr h_tr ⟨lhs, rhs, ⟨ h_out, h_inputs ⟩⟩
+    subst h_out
+    simp [Kleene.Forall] at h_inputs
+    simp [Bytes.Publishable]
+    grind
+
+instance: SubAttackerKnowledgeTheorem attKnowsSplitLeft where
+  pf := by
+    simp only [attKnowsSplitLeft]
+    intro out tr h_tr ⟨inp, rhs, i, ⟨ h_out, h_inputs ⟩⟩
+    simp [Kleene.Forall] at h_inputs
+    simp [Bytes.Publishable]
+    have := split.label inp i tr
+    have := split.Invariant inp i tr
+    grind
+
+instance: SubAttackerKnowledgeTheorem attKnowsSplitRight where
+  pf := by
+    simp only [attKnowsSplitRight]
+    intro out tr h_tr ⟨inp, lhs, i, ⟨ h_out, h_inputs ⟩⟩
+    simp [Kleene.Forall] at h_inputs
+    simp [Bytes.Publishable]
+    have := split.label inp i tr
+    have := split.Invariant inp i tr
+    grind
+
+instance: ∀ id, SubAttackerKnowledgeTheorem (attackerKnowledge.internal id)
+  | 0 => inferInstanceAs (SubAttackerKnowledgeTheorem attKnowsConcat)
+  | 1 => inferInstanceAs (SubAttackerKnowledgeTheorem attKnowsSplitLeft)
+  | 2 => inferInstanceAs (SubAttackerKnowledgeTheorem attKnowsSplitRight)
+
+public
+instance: SubAttackerKnowledgeTheorem attackerKnowledge := inferInstanceAs (SubAttackerKnowledgeTheorem (SubAttackerKnowledge.combine' attackerKnowledge.internal))
+
+end AttackerKnowledgeTheorem
+
+end DY.Concat
