DY/EquationalTheory/Hash.lean
@@ -1,0 +1,185 @@
+module
+
+public import DY.Bytes
+public import DY.Misc.Instances
+
+namespace DY.Hash
+
+public
+class CanHash (Bytes: Type u) where
+  hash: Bytes → Bytes
+
+export CanHash (hash)
+
+section Constructors
+
+public
+structure Hash (Bytes: Type) where
+  input: Bytes
+
+public
+instance: ALaCarte.FunctorSizeOf Hash where
+  sizeOf | {input} => sizeOf input
+
+public
+instance: ALaCarte.Representable Hash where
+  CtorId := Unit
+  ctors | () => { Data := Unit, nRec := 1 }
+
+  toRepr | {input} => {
+    id := ()
+    data := ()
+    as := #v[input]
+  }
+  fromRepr
+  | {id, data, as} =>
+    let input := as[0]
+    { input }
+  from_to | {input} => by rfl
+  to_from
+  | {id, data, as} => by
+    simp_all <;> grind
+  sizeOf_eq | {input} => by simp +arith [ALaCarte.FunctorSizeOf.sizeOf]
+
+public instance: ALaCarte.RepresentableDecidableEq Hash where
+public instance: ALaCarte.RepresentableOrd Hash where
+public instance: SubBytesFunctor Hash where
+
+public
+abbrev SubF := Hash
+
+public
+def Hash.length [BytesFunctor]: Bytes.PartialLength Hash :=
+  fun _ _ =>
+    32
+
+public
+abbrev SubF.length [BytesFunctor]: Bytes.PartialLength SubF := Hash.length
+
+variable [BytesFunctor] [BytesFunctor.Has SubF]
+
+public
+abbrev Hash.pack (x: Hash Bytes) := BytesView.pack x
+
+public
+instance: CanHash Bytes where
+  hash input := ({input}: Hash Bytes).pack
+
+public
+theorem hash_inj
+  (inp1 inp2: Bytes)
+  :
+    hash inp1 = hash inp2 →
+    inp1 = inp2
+:= by
+  simp only [hash]
+  grind
+
+end Constructors
+
+section AttackerKnowledge
+
+variable [BytesFunctor] [BytesFunctor.Has SubF]
+
+public
+def attKnowsHash: SubAttackerKnowledge Hash where
+  pred p out :=
+    ∃ inp,
+      out = hash inp ∧
+      p inp
+
+public
+abbrev attackerKnowledge := attKnowsHash
+
+variable [AttackerKnowledge] [AttackerKnowledge.Has attackerKnowledge]
+
+public
+theorem attacker_knows_hash
+  (inp: Bytes) (tr: Trace α)
+  : inp.AttackerKnows tr →
+    (hash inp).AttackerKnows tr
+:= by
+  intro h_inp
+  apply Bytes.AttackerKnows.prove attKnowsHash
+  simp only [attKnowsHash]
+  grind
+
+end AttackerKnowledge
+
+section Invariants
+
+variable [BytesFunctor] [BytesFunctor.Has SubF]
+
+public
+def Hash.invariants: Bytes.PartialInvariants Hash where
+  well_formed := fun {input := input} rec tr =>
+    (rec input) tr
+
+  usage := fun {input := input} rec tr => Usage.nothing
+
+  label := fun {input := input} rec tr =>
+    (rec input) tr
+
+  invariant := fun {input := input} rec tr =>
+    (rec input) tr
+
+public
+abbrev invariants: Bytes.PartialInvariants SubF := Hash.Hash.invariants
+
+public
+def Hash.invariantsProofs [BytesInvariants]: Bytes.PartialInvariantsProofs Hash.invariants where
+
+public
+abbrev invariantsProofs [BytesInvariants]: Bytes.PartialInvariantsProofs invariants := Hash.Hash.invariantsProofs
+
+variable [BytesInvariants] [BytesInvariants.Has invariants]
+
+@[simp]
+public
+theorem hash.WellFormed
+  (inp: Bytes) (tr: ProofTrace)
+  :
+    (hash inp).WellFormed tr = inp.WellFormed tr
+:= by
+  simp [hash, Bytes.WellFormed.eq, Hash.invariants]
+
+@[simp]
+public
+theorem hash.label
+  (inp: Bytes) (tr: ProofTrace)
+  : (hash inp).label tr = inp.label tr
+:= by
+  simp [hash, Bytes.label.eq, Hash.invariants]
+
+@[simp]
+public
+theorem hash.Invariant
+  (inp: Bytes) (tr: ProofTrace)
+  :
+    (hash inp).Invariant tr =
+    inp.Invariant tr
+:= by
+  simp [hash, Bytes.Invariant.eq, Hash.invariants]
+
+end Invariants
+
+section AttackerKnowledgeTheorem
+
+variable [BytesFunctor] [BytesInvariants]
+variable [BytesFunctor.Has SubF]
+variable [BytesInvariants.Has invariants]
+
+public
+instance: SubAttackerKnowledgeTheorem attKnowsHash where
+  pf := by
+    simp only [attKnowsHash]
+    intro out tr h_tr ⟨inp, ⟨ h_out, h_inp ⟩⟩
+    subst h_out
+    simp_all [Bytes.Publishable]
+
+public
+example: SubAttackerKnowledgeTheorem attackerKnowledge := inferInstance
+
+end AttackerKnowledgeTheorem
+
+end DY.Hash
