DY/EquationalTheory/Literal.lean
@@ -1,0 +1,199 @@
+module
+
+public import DY.Bytes
+public import DY.Misc.Instances
+
+namespace DY.Literal
+
+public
+class CanMkLiteral (Bytes: Type u) where
+  literalToBytes: ByteArray → Bytes
+  bytesToLiteral: Bytes → Option ByteArray
+
+export CanMkLiteral (literalToBytes)
+export CanMkLiteral (bytesToLiteral)
+
+-- Constructors
+
+section Constructors
+
+public
+structure Literal (Bytes: Type) where
+  lit: ByteArray
+
+public
+instance: ALaCarte.FunctorSizeOf Literal where
+  sizeOf | {lit := _} => 0
+
+public
+instance: ALaCarte.Representable Literal where
+  CtorId := Unit
+  ctors | () => { Data := ByteArray, nRec := 0 }
+
+  toRepr | {lit} => {
+    id := ()
+    data := lit
+    as := #v[]
+  }
+  fromRepr
+  | {id, data := lit, as} =>
+    { lit }
+  from_to | {lit} => by rfl
+  to_from
+  | {id, data, as} => by
+    simp_all <;> grind
+  sizeOf_eq | {lit := _} => by simp +arith [ALaCarte.FunctorSizeOf.sizeOf]
+
+public instance: ALaCarte.RepresentableDecidableEq Literal where
+public instance: ALaCarte.RepresentableOrd Literal where
+
+public instance: SubBytesFunctor Literal where
+
+public
+abbrev SubF := Literal
+
+public
+def Literal.length [BytesFunctor]: Bytes.PartialLength Literal :=
+  fun { lit := lit } _ =>
+    lit.size
+
+public
+abbrev SubF.length [BytesFunctor]: Bytes.PartialLength SubF := Literal.length
+
+public
+abbrev Literal.pack [BytesFunctor] [BytesFunctor.Has SubF] (x: Literal Bytes) := BytesView.pack x
+
+public
+instance [BytesFunctor] [BytesFunctor.Has SubF]: CanMkLiteral Bytes where
+  literalToBytes lit :=
+    ({ lit }: Literal Bytes).pack
+
+  bytesToLiteral buf :=
+    match buf.view? Literal with
+    | some { lit } =>
+      some lit
+    | none => none
+
+public
+theorem bytesToLiteral_literalToBytes
+  [BytesFunctor] [BytesFunctor.Has SubF]
+  (lit: ByteArray)
+  : bytesToLiteral (literalToBytes lit: Bytes) = some lit
+:= by
+  simp only [bytesToLiteral, literalToBytes]
+  grind
+
+public
+theorem literalToBytes_bytesToLiteral
+  [BytesFunctor] [BytesFunctor.Has SubF]
+  (buf: Bytes)
+  : match bytesToLiteral buf with
+    | none => True
+    | some lit =>
+      buf = literalToBytes lit
+:= by
+  simp only [bytesToLiteral, literalToBytes]
+  grind
+
+end Constructors
+
+section AttackerKnowledge
+
+variable [BytesFunctor] [BytesFunctor.Has SubF]
+
+public
+def attKnowsLit: SubAttackerKnowledge Literal where
+  pred p out :=
+    ∃ lit,
+      out = literalToBytes lit
+
+public
+abbrev attackerKnowledge := attKnowsLit
+
+variable [AttackerKnowledge] [AttackerKnowledge.Has attackerKnowledge]
+
+public
+theorem attacker_knows_literalToBytes
+  (lit: ByteArray) (tr: Trace α)
+  : (literalToBytes lit: Bytes).AttackerKnows tr
+:= by
+  apply Bytes.AttackerKnows.prove attKnowsLit
+  simp only [attKnowsLit]
+  exists lit
+
+end AttackerKnowledge
+
+section Invariants
+
+variable [BytesFunctor] [BytesFunctor.Has SubF]
+
+public
+def Literal.invariants: Bytes.PartialInvariants Literal where
+  well_formed := fun {lit := _} _rec _tr =>
+    True
+
+  usage := fun {lit := _} _rec _tr => Usage.nothing
+
+  label := fun {lit := _} _rec _tr =>
+    Label.pub
+
+  invariant := fun {lit := _} _rec _tr =>
+    True
+
+public
+abbrev invariants: Bytes.PartialInvariants SubF := Literal.Literal.invariants
+
+public
+def Literal.invariantsProofs [BytesInvariants]: Bytes.PartialInvariantsProofs Literal.invariants where
+
+public
+abbrev invariantsProofs [BytesInvariants]: Bytes.PartialInvariantsProofs invariants := Literal.Literal.invariantsProofs
+
+variable [BytesInvariants] [BytesInvariants.Has invariants]
+
+@[simp]
+public
+theorem literalToBytes.WellFormed
+  (lit: ByteArray) (tr: ProofTrace)
+  : (literalToBytes lit: Bytes).WellFormed tr
+:= by
+  simp [literalToBytes, Bytes.WellFormed.eq, Literal.invariants]
+
+@[simp]
+public
+theorem literalToBytes.label
+  (lit: ByteArray) (tr: ProofTrace)
+  : (literalToBytes lit: Bytes).label tr = Label.pub
+:= by
+  simp [literalToBytes, Bytes.label.eq, Literal.invariants]
+
+@[simp]
+public
+theorem literalToBytes.Invariant
+  (lit: ByteArray) (tr: ProofTrace)
+  : (literalToBytes lit: Bytes).Invariant tr
+:= by
+  simp [literalToBytes, Bytes.Invariant.eq, Literal.invariants]
+
+end Invariants
+
+section AttackerKnowledgeTheorem
+
+variable [BytesFunctor] [BytesInvariants]
+variable [BytesFunctor.Has SubF]
+variable [BytesInvariants.Has invariants]
+
+public
+instance: SubAttackerKnowledgeTheorem attKnowsLit where
+  pf := by
+    simp only [attKnowsLit]
+    intro out tr h_tr ⟨lit, h_out⟩
+    subst h_out
+    simp [Bytes.Publishable]
+    grind
+
+example: SubAttackerKnowledgeTheorem attackerKnowledge := inferInstance
+
+end AttackerKnowledgeTheorem
+
+end DY.Literal
