DY/EquationalTheory/Sign.lean
@@ -1,0 +1,582 @@
+module
+
+public import DY.Bytes
+public import DY.Misc.Instances
+
+namespace DY.Signature
+
+public
+class CanSign (Bytes: Type u) where
+  vk: (sk: Bytes) → Bytes
+  sign: (sk: Bytes) → (nonce: Bytes) → (msg: Bytes) → Bytes
+  verify: (vk: Bytes) → (msg: Bytes) → (sig: Bytes) → Bool
+
+export CanSign (vk)
+export CanSign (sign)
+export CanSign (verify)
+
+section Constructors
+
+public
+structure Vk (Bytes: Type) where
+  sk: Bytes
+
+public
+instance: ALaCarte.FunctorSizeOf Vk where
+  sizeOf | {sk} => sizeOf sk
+
+public
+instance: ALaCarte.Representable Vk where
+  CtorId := Unit
+  ctors | () => { Data := Unit, nRec := 1 }
+
+  toRepr | {sk} => {
+    id := ()
+    data := ()
+    as := #v[sk]
+  }
+  fromRepr
+  | {id, data, as} =>
+    let sk := as[0]
+    { sk }
+  from_to | {sk} => by rfl
+  to_from
+  | {id, data, as} => by
+    simp_all <;> grind
+  sizeOf_eq | {sk} => by simp +arith [ALaCarte.FunctorSizeOf.sizeOf]
+
+public instance: ALaCarte.RepresentableDecidableEq Vk where
+public instance: ALaCarte.RepresentableOrd Vk where
+public instance: SubBytesFunctor Vk where
+
+public
+def Vk.length [BytesFunctor]: Bytes.PartialLength Vk :=
+  fun _ _ =>
+    32
+
+public
+structure Sign (Bytes: Type) where
+  sk: Bytes
+  nonce: Bytes
+  msg: Bytes
+
+public
+instance: ALaCarte.FunctorSizeOf Sign where
+  sizeOf | {sk, nonce, msg} => sizeOf sk + sizeOf nonce + sizeOf msg
+
+public
+instance: ALaCarte.Representable Sign where
+  CtorId := Unit
+  ctors | () => { Data := Unit, nRec := 3 }
+
+  toRepr | {sk, nonce, msg} => {
+    id := ()
+    data := ()
+    as := #v[sk, nonce, msg]
+  }
+  fromRepr
+  | {id, data, as} =>
+    let sk := as[0]
+    let nonce := as[1]
+    let msg := as[2]
+    { sk, nonce, msg }
+  from_to | {sk, nonce, msg} => by rfl
+  to_from
+  | {id, data, as} => by
+    simp_all <;> grind
+  sizeOf_eq | {sk, nonce, msg} => by simp +arith [ALaCarte.FunctorSizeOf.sizeOf]
+
+public instance: ALaCarte.RepresentableDecidableEq Sign where
+public instance: ALaCarte.RepresentableOrd Sign where
+public instance: SubBytesFunctor Sign where
+
+public
+def Sign.length [BytesFunctor]: Bytes.PartialLength Sign :=
+  fun _ _ =>
+    64
+
+public
+abbrev SubF.internal (id: Fin 2): Type → Type :=
+  match id with
+  | 0 => Vk
+  | 1 => Sign
+
+public
+abbrev SubF := BytesFunctor.combine SubF.internal
+
+public
+instance: ∀ id, SubBytesFunctor (SubF.internal id)
+  | 0 => inferInstance
+  | 1 => inferInstance
+
+public
+instance: SubBytesFunctor SubF := inferInstance
+
+public instance: BytesFunctor.HasStep Vk SubF := inferInstanceAs (BytesFunctor.HasStep (SubF.internal 0) SubF)
+public instance: BytesFunctor.HasStep Sign SubF := inferInstanceAs (BytesFunctor.HasStep (SubF.internal 1) SubF)
+
+public
+def SubF.length.internal [BytesFunctor]: ∀ id, Bytes.PartialLength (SubF.internal id)
+  | 0 => Vk.length
+  | 1 => Sign.length
+
+public
+abbrev SubF.length [BytesFunctor]: Bytes.PartialLength SubF :=
+  Bytes.PartialLength.combine SubF.length.internal
+
+public instance [BytesFunctor] [BytesLength]: BytesLength.HasStep Vk.length SubF.length := inferInstanceAs (BytesLength.HasStep (SubF.length.internal 0) SubF.length)
+public instance [BytesFunctor] [BytesLength]: BytesLength.HasStep Sign.length SubF.length := inferInstanceAs (BytesLength.HasStep (SubF.length.internal 1) SubF.length)
+
+variable [BytesFunctor] [BytesFunctor.Has SubF]
+
+public abbrev Vk.pack (x: Vk Bytes) := BytesView.pack x
+public abbrev Sign.pack (x: Sign Bytes) := BytesView.pack x
+
+public
+instance: CanSign Bytes where
+  vk sk :=
+    ({sk}: Vk Bytes).pack
+
+  sign sk nonce msg :=
+    ({sk, nonce, msg}: Sign Bytes).pack
+
+  verify vk msg sig :=
+    match sig.view? Sign with
+    | some { sk, nonce := _, msg := msg' } =>
+      msg = msg' &&
+      vk = ({sk} : Vk Bytes).pack
+    | none => false
+
+public
+theorem verify_sign
+  (sk nonce msg: Bytes)
+  : verify (vk sk) msg (sign sk nonce msg) = true
+:= by
+  simp only [verify, vk, sign]
+  grind
+
+end Constructors
+
+section AttackerKnowledge
+
+variable [BytesFunctor] [BytesFunctor.Has SubF]
+
+def attKnowsVk: SubAttackerKnowledge SubF where
+  pred p out :=
+    ∃ sk,
+      out = vk sk ∧
+      p sk
+
+def attKnowsSign: SubAttackerKnowledge SubF where
+  pred p out :=
+    ∃ sk nonce msg,
+      out = sign sk nonce msg ∧
+      Kleene.Forall p [sk, nonce, msg]
+
+def attackerKnowledge.internal (id: Fin 2): SubAttackerKnowledge SubF :=
+  match id with
+  | 0 => attKnowsVk
+  | 1 => attKnowsSign
+
+public
+def attackerKnowledge: SubAttackerKnowledge SubF :=
+  SubAttackerKnowledge.combine' attackerKnowledge.internal
+
+instance: AttackerKnowledge.HasStep attKnowsVk attackerKnowledge := inferInstanceAs (AttackerKnowledge.HasStep (attackerKnowledge.internal 0) (SubAttackerKnowledge.combine' attackerKnowledge.internal))
+instance: AttackerKnowledge.HasStep attKnowsSign attackerKnowledge := inferInstanceAs (AttackerKnowledge.HasStep (attackerKnowledge.internal 1) (SubAttackerKnowledge.combine' attackerKnowledge.internal))
+
+variable [AttackerKnowledge] [AttackerKnowledge.Has attackerKnowledge]
+
+public
+theorem attacker_knows_vk
+  (sk: Bytes) (tr: Trace α)
+  : sk.AttackerKnows tr →
+    (vk sk).AttackerKnows tr
+:= by
+  intro h_inp
+  apply Bytes.AttackerKnows.prove attKnowsVk
+  simp only [attKnowsVk]
+  grind
+
+public
+theorem attacker_knows_sign
+  (sk nonce msg: Bytes) (tr: Trace α)
+  : sk.AttackerKnows tr →
+    nonce.AttackerKnows tr →
+    msg.AttackerKnows tr →
+    (sign sk nonce msg).AttackerKnows tr
+:= by
+  intro h_inp h_nonce h_msg
+  apply Bytes.AttackerKnows.prove attKnowsSign
+  simp only [attKnowsSign, Kleene.Forall]
+  grind
+
+end AttackerKnowledge
+
+section Invariants
+
+variable [BytesFunctor] [BytesFunctor.Has SubF]
+
+public
+def Vk.invariants: Bytes.PartialInvariants Vk where
+  well_formed := fun {sk := sk} rec tr =>
+    (rec sk) tr
+
+  usage := fun {sk := sk} rec tr =>
+    Usage.nothing
+
+  label := fun {sk := sk} rec tr =>
+    Label.pub
+
+  invariant := fun {sk := sk} rec tr =>
+    (rec sk) tr
+
+public
+def Vk.invariantsProofs [BytesInvariants]: Bytes.PartialInvariantsProofs Vk.invariants where
+
+section VkLemmas
+
+variable [BytesInvariants] [BytesInvariants.Has Vk.invariants]
+
+@[simp]
+public
+theorem vk.WellFormed
+  (inp: Bytes) (tr: ProofTrace)
+  : (vk inp).WellFormed tr = inp.WellFormed tr
+:= by
+  simp [vk, Bytes.WellFormed.eq, Vk.invariants]
+
+@[simp]
+public
+theorem vk.label
+  (inp: Bytes) (tr: ProofTrace)
+  : (vk inp).label tr = Label.pub
+:= by
+  simp [vk, Bytes.label.eq, Vk.invariants]
+
+@[simp]
+public
+theorem vk.Invariant
+  (inp: Bytes) (tr: ProofTrace)
+  : inp.Invariant tr →
+    (vk inp).Invariant tr
+:= by
+  simp [vk, Bytes.Invariant.eq, Vk.invariants]
+
+end VkLemmas
+
+public
+class SignPred where
+  pred: [GetUsage] → [GetLabel] → Usage → Bytes → Bytes → ProofTrace → Prop
+
+public
+class SignPredProof [BytesInvariants] [SignPred] where
+  pred_later:
+    [BytesWellFormedLater] → [GetUsageLater] → [GetLabelLater] →
+    ∀ skUsg vk msg tr1 tr2,
+      vk.WellFormed tr1 →
+      msg.WellFormed tr1 →
+      tr1 ≤ tr2 →
+      SignPred.pred skUsg vk msg tr1 →
+      SignPred.pred skUsg vk msg tr2
+
+grind_pattern SignPredProof.pred_later => tr1 ≤ tr2, SignPred.pred skUsg vk msg tr1
+
+public
+def Sign.invariants [SignPred]: Bytes.PartialInvariants Sign where
+  well_formed := fun {sk, nonce, msg} rec tr =>
+      (rec sk) tr ∧
+      (rec nonce) tr ∧
+      (rec msg) tr
+
+  usage := fun {sk, nonce, msg} rec tr =>
+    Usage.nothing
+
+  label := fun {sk, nonce, msg} rec tr =>
+    (rec msg) tr
+
+  invariant := fun {sk, nonce, msg} rec tr =>
+      (rec sk) tr ∧
+      (rec nonce) tr ∧
+      (rec msg) tr ∧
+      (
+        (
+          exists sk_usg,
+          -- Honest case:
+          -- - the key has the usage of signature key
+          sk.HasUsage sk_usg tr ∧
+          sk_usg.type = "SigKey" ∧
+          -- - the custom (protocol-specific) invariant hold (authentication)
+          SignPred.pred sk_usg (vk sk) msg tr ∧
+          -- - the nonce is more secret than the signature key
+          --   (this is because the standard EUF-CMA security assumption on signatures
+          --   do not have any guarantees when the nonce is leaked to the attacker,
+          --   in practice knowing the nonce used to sign a message
+          --   can be used to obtain the private key,
+          --   hence this restriction)
+          (sk.label tr).canFlow (nonce.label tr) tr ∧
+          -- - the nonce has the correct usage (for the same reason as above)
+          -- nonce `has_usage tr` SigNonce
+          True
+        ) ∨ (
+          -- Attacker case:
+          -- the attacker knows the signature key.
+          -- The message is not required to be known by the attacker:
+          -- the EUF-CMA security assumption on signatures doesn't guarantee
+          -- that in case of signature forgeries.
+          (sk.label tr).canFlow Label.pub tr
+        )
+      )
+
+public
+def Sign.invariantsProofs [BytesInvariants] [BytesInvariants.Has Vk.invariants] [SignPred] [SignPredProof]: Bytes.PartialInvariantsProofs Sign.invariants where
+  invariant_later := by
+    intro _ _ _ _ x rec tr1 tr2
+    cases x
+    simp_all [invariants, DY.ALaCarte.FunctorSizeOf.sizeOf, BytesInvariantLaterT]
+    -- TODO: grind set
+    grind [vk.WellFormed]
+
+public
+def invariants.internal [SignPred]: (id: Fin 2) → Bytes.PartialInvariants (SubF.internal id)
+  | 0 => Vk.invariants
+  | 1 => Sign.invariants
+
+public
+abbrev invariants [SignPred]: Bytes.PartialInvariants SubF :=
+  Bytes.PartialInvariants.combine invariants.internal
+
+public instance [BytesInvariants] [SignPred]: BytesInvariants.HasStep Vk.invariants invariants := inferInstanceAs (BytesInvariants.HasStep (invariants.internal 0) invariants)
+public instance [BytesInvariants] [SignPred]: BytesInvariants.HasStep Sign.invariants invariants := inferInstanceAs (BytesInvariants.HasStep (invariants.internal 1) invariants)
+
+def invariantsProofs.internal [BytesInvariants] [BytesInvariants.Has Vk.invariants] [SignPred] [SignPredProof]: (id: Fin 2) → Bytes.PartialInvariantsProofs (invariants.internal id)
+  | 0 => Vk.invariantsProofs
+  | 1 => Sign.invariantsProofs
+
+public
+def invariantsProofs [BytesInvariants] [BytesInvariants.Has Vk.invariants] [SignPred] [SignPredProof]: Bytes.PartialInvariantsProofs invariants :=
+  Bytes.PartialInvariantsProofs.combine invariantsProofs.internal
+
+end Invariants
+
+-- Temporarly close the namespace to define Bytes.SignkeyHasUsage and Bytes.signkeyLabel
+end Signature
+
+section ExtractSignKey
+
+variable [BytesFunctor]
+variable [BytesFunctor.Has Signature.SubF]
+
+noncomputable
+def Signature.extractSignkey (vk: Bytes): Option Bytes :=
+  match vk.view? Signature.Vk with
+  | some { sk } =>
+    some sk
+  | none => none
+
+theorem Signature.vk_extractSignkey (b: Bytes):
+  match extractSignkey b with
+  | none => True
+  | some sk => b = Signature.vk sk
+:= by
+  simp [extractSignkey, Signature.vk]
+  grind
+
+theorem Signature.extractSignkey.preserves_WellFormed
+  [BytesInvariants] [Signature.SignPred] [BytesInvariants.Has Signature.invariants]
+: ExtractPreservesWellFormed extractSignkey
+:= by
+  simp [ExtractPreservesWellFormed]
+  grind [Signature.vk_extractSignkey, Signature.vk.WellFormed]
+
+public
+def Bytes.SignkeyHasUsage
+  [BytesInvariants]
+  (vk: Bytes) (skUsg: Usage) (tr: ProofTrace): Prop
+:=
+  Bytes.XXXHasUsage Signature.extractSignkey vk skUsg tr
+
+public
+theorem Bytes.SignkeyHasUsage_vk
+  [BytesInvariants]
+  (sk: Bytes) (skUsg: Usage) (tr: ProofTrace)
+  : (Signature.vk sk).SignkeyHasUsage skUsg tr = sk.HasUsage skUsg tr
+:= by
+  simp [Bytes.SignkeyHasUsage, Bytes.XXXHasUsage, Signature.extractSignkey, Signature.vk]
+  grind
+
+grind_pattern Bytes.SignkeyHasUsage_vk => (Signature.vk sk).SignkeyHasUsage skUsg tr
+
+public
+theorem Bytes.SignkeyHasUsage_later
+  [BytesInvariants] [BytesInvariantsProofs]
+  [Signature.SignPred] [BytesInvariants.Has Signature.invariants]
+  (b: Bytes) (usg: Usage) (tr1 tr2: ProofTrace)
+  : b.WellFormed tr1 →
+    tr1 ≤ tr2 →
+    b.SignkeyHasUsage usg tr1 →
+    b.SignkeyHasUsage usg tr2
+:= by
+  simp [Bytes.SignkeyHasUsage]
+  apply Bytes.XXXHasUsage_later Signature.extractSignkey Signature.extractSignkey.preserves_WellFormed
+
+grind_pattern Bytes.SignkeyHasUsage_later => tr1 ≤ tr2, b.SignkeyHasUsage usg tr1
+
+public
+noncomputable
+def Bytes.signkeyLabel
+  [BytesInvariants]
+  (vk: Bytes) (tr: ProofTrace): Label
+:=
+  Bytes.xxxLabel Signature.extractSignkey vk tr
+
+public
+theorem Bytes.signkeyLabel_vk
+  [BytesInvariants]
+  [Signature.SignPred] [BytesInvariants.Has Signature.invariants]
+  (sk: Bytes) (tr: ProofTrace)
+  : (Signature.vk sk).signkeyLabel tr = sk.label tr
+:= by
+  simp [Bytes.signkeyLabel, Bytes.xxxLabel, Signature.extractSignkey, Signature.vk]
+  grind
+
+grind_pattern Bytes.signkeyLabel_vk => (Signature.vk sk).signkeyLabel tr
+
+public
+theorem Bytes.signkeyLabel_later
+  [BytesInvariants] [BytesInvariantsProofs]
+  [Signature.SignPred] [BytesInvariants.Has Signature.invariants]
+  (b: Bytes) (tr1 tr2: ProofTrace)
+  : b.WellFormed tr1 →
+    tr1 ≤ tr2 →
+    b.signkeyLabel tr1 = b.signkeyLabel tr2
+:= by
+  simp [Bytes.signkeyLabel]
+  apply Bytes.xxxLabel_later Signature.extractSignkey Signature.extractSignkey.preserves_WellFormed
+
+grind_pattern Bytes.signkeyLabel_later => tr1 ≤ tr2, b.signkeyLabel tr1
+
+end ExtractSignKey
+
+namespace Signature
+
+section Invariants
+
+variable [BytesFunctor] [BytesFunctor.Has SubF]
+
+variable [SignPred]
+variable [BytesInvariants]
+variable [BytesInvariants.Has invariants]
+
+@[simp]
+public
+theorem sign.WellFormed
+  (sk nonce msg: Bytes) (tr: ProofTrace)
+  : (sign sk nonce msg).WellFormed tr = (
+      sk.WellFormed tr ∧
+      nonce.WellFormed tr ∧
+      msg.WellFormed tr
+    )
+:= by
+  simp [sign, Bytes.WellFormed.eq, Sign.invariants]
+
+@[simp]
+public
+theorem sign.label
+  (sk nonce msg: Bytes) (tr: ProofTrace)
+  : (sign sk nonce msg).label tr = msg.label tr
+:= by
+  simp [sign, Bytes.label.eq, Sign.invariants]
+
+@[simp]
+public
+theorem sign.Invariant
+  (sk nonce msg: Bytes) (sk_usg: Usage) (tr: ProofTrace)
+  : (
+      sk.Invariant tr ∧
+      nonce.Invariant tr ∧
+      msg.Invariant tr ∧
+      sk.HasUsage sk_usg tr ∧
+      --nonce `has_usage tr` SigNonce /\
+      (sk.label tr).canFlow (nonce.label tr) tr ∧
+      (
+        (
+          sk_usg.type = "SigKey" ∧
+          SignPred.pred sk_usg (vk sk) msg tr
+        ) ∨ (
+          (sk.label tr).canFlow Label.pub tr
+        )
+      )
+    ) →
+    (sign sk nonce msg).Invariant tr
+:= by
+  have := vk.WellFormed sk tr
+  simp [sign, Bytes.Invariant.eq, Sign.invariants]
+  grind
+
+@[simp]
+public
+theorem verify.Invariant
+  (vk msg sig: Bytes) (skUsg: Usage) (tr: ProofTrace)
+  : vk.Invariant tr →
+    msg.Invariant tr →
+    sig.Invariant tr →
+    vk.SignkeyHasUsage skUsg tr →
+    verify vk msg sig → (
+      (
+        skUsg.type = "SigKey" →
+        SignPred.pred skUsg vk msg tr
+      ) ∨ (
+        (vk.signkeyLabel tr).canFlow Label.pub tr
+      )
+    )
+:= by
+  simp [verify]
+  split
+  · rename_i sk nonce msg heq
+    have := Bytes.pack_view? Sign sig
+    simp only [heq] at this
+    subst this
+    have: ({sk}: Vk Bytes).pack = CanSign.vk sk := rfl
+    have := Bytes.HasUsage_inj sk skUsg
+    simp_all [Bytes.Invariant.eq, Sign.invariants]
+    grind
+  · simp
+
+end Invariants
+
+section AttackerKnowledgeTheorem
+
+variable [BytesFunctor] [BytesInvariants]
+variable [BytesFunctor.Has SubF]
+variable [SignPred]
+variable [BytesInvariants.Has invariants]
+
+-- Preserve publishability
+
+instance: SubAttackerKnowledgeTheorem attKnowsVk where
+  pf := by
+    simp only [attKnowsVk]
+    intro out tr h_tr ⟨sk, ⟨ h_out, h_sk ⟩⟩
+    subst h_out
+    simp_all [Bytes.Publishable]
+    grind
+
+instance: SubAttackerKnowledgeTheorem attKnowsSign where
+  pf := by
+    simp only [attKnowsSign]
+    intro out tr h_tr ⟨sk, nonce, msg, ⟨ h_out, h_inputs ⟩⟩
+    subst h_out
+    simp_all [Bytes.Publishable, Kleene.Forall]
+    simp [sign, Bytes.Invariant.eq, Sign.invariants]
+    grind
+
+instance: ∀ id, SubAttackerKnowledgeTheorem (attackerKnowledge.internal id)
+  | 0 => inferInstanceAs (SubAttackerKnowledgeTheorem attKnowsVk)
+  | 1 => inferInstanceAs (SubAttackerKnowledgeTheorem attKnowsSign)
+
+public instance: SubAttackerKnowledgeTheorem attackerKnowledge := inferInstanceAs (SubAttackerKnowledgeTheorem (SubAttackerKnowledge.combine' attackerKnowledge.internal))
+
+end AttackerKnowledgeTheorem
+
+end DY.Signature
